{
 "cells": [
  {
   "cell_type": "markdown",
   "metadata": {},
   "source": [
    "# Vecor Calculus\n",
    "## 5.1\n",
    "Using intermediate variables and flow chart:  \n",
    "$$a = x^4 \\quad \\quad c = x^3$$\n",
    "$$b = log(a) \\quad \\quad d = sin(c)$$\n",
    "$$f = bd$$\n",
    "\n",
    "![5.1](../Images/Screenshot%202023-08-01%20at%2012.01.20%20PM.png)\n",
    "\n",
    "We want: \n",
    "\n",
    "$$ \n",
    "\\begin{aligned}\n",
    "{\\partial f \\over \\partial x} &= {\\partial f \\over \\partial b}{\\partial b \\over \\partial x} + {\\partial f \\over \\partial d}{\\partial d \\over \\partial x} \\\\\n",
    "&= {\\partial f \\over \\partial b}{\\partial b \\over \\partial a}{\\partial a \\over \\partial x} + {\\partial f \\over \\partial d}{\\partial d \\over \\partial c}{\\partial c \\over \\partial x}\n",
    "\\end{aligned}\n",
    "$$\n",
    "\n",
    "First derive all elementary derivatives:\n",
    "$${\\partial a \\over \\partial x} = 4x^3 \\quad \\quad {\\partial c \\over \\partial x} = 3x^2 $$ \n",
    "$${\\partial b \\over \\partial a} = {1 \\over a} \\quad \\quad {\\partial d \\over \\partial c} = cos(c)$$\n",
    "$${\\partial f \\over \\partial b} = d \\quad \\quad {\\partial f \\over \\partial d} = b$$\n",
    "\n",
    "Then by backward propagation, we calculate the derivative products in *reverse* of the flow chart direction.\n",
    "$$\n",
    "{\\partial f \\over \\partial a} = {\\partial f \\over \\partial b}{\\partial b \\over \\partial a} = {d \\over a}\n",
    "$$\n",
    "$$\n",
    "{\\partial f \\over \\partial c} = {\\partial f \\over \\partial d}{\\partial d \\over \\partial c} = {bcos(c)}\n",
    "$$\n",
    "So \n",
    "$$\n",
    "\\begin{aligned}\n",
    "{\\partial f \\over \\partial x} &= {\\partial f \\over \\partial a}{\\partial a \\over \\partial x} + {\\partial f \\over \\partial c}{\\partial c \\over \\partial x} \\\\\n",
    "&= {d\\over a}{4x^3} + bcos(c) 3x^2 \\\\\n",
    "&= {sin(x^3)\\over x^4}{4x^3} + log(x^4)cos(x^3)3x^2 \\\\\n",
    "&= {4\\over x}{sin(x^3)} + 12x^2log(x)cos(x^3)\n",
    "\\end{aligned}\n",
    "$$\n"
   ]
  },
  {
   "cell_type": "markdown",
   "metadata": {},
   "source": [
    "\n",
    "## 5.2\n",
    "Let \n",
    "$$\n",
    "\\begin{aligned}\n",
    "&a = -x \\quad \\quad &b = e^a \\\\\n",
    "&c =1+b \\quad \\quad &f = {1\\over c}\n",
    "\\end{aligned}\n",
    "$$\n",
    "\n",
    "$$\n",
    "\\begin{aligned}\n",
    "{\\partial f \\over \\partial x} &= {\\partial f \\over \\partial c}{\\partial c \\over \\partial b}{\\partial b \\over \\partial a}{\\partial a \\over \\partial x} \\\\\n",
    "&= {\\left(-{1 \\over {c^2}} \\cdot 1\\right)}{\\partial b \\over \\partial a}{\\partial a \\over \\partial x} \\\\\n",
    "&= {\\left(-{1 \\over {c^2}} \\cdot e^a\\right)}{\\partial a \\over \\partial x} \\\\\n",
    "&= -{{e^a \\over c^2} \\cdot {(-1)}} = {e^a \\over c^2} \\\\\n",
    "&= {{e^{-x}} \\over \\left(1+e^{-x}\\right)^2}\n",
    "\\end{aligned}\n",
    "$$\n"
   ]
  },
  {
   "cell_type": "markdown",
   "metadata": {},
   "source": [
    "\n",
    "## 5.3\n",
    "Let $a = x-u, b=a^2, c = -{1 \\over {2\\sigma^2}}b, f = exp(c)$, then\n",
    "$$\n",
    "\\begin{aligned}\n",
    "{\\partial f \\over \\partial x} &= {\\partial f \\over \\partial c}{\\partial c \\over \\partial b}{\\partial b \\over \\partial a}{\\partial a \\over \\partial x} \\\\\n",
    "&= \\left(e^c \\cdot -{1 \\over {2\\sigma^2}}\\right){\\partial b \\over \\partial a}{\\partial a \\over \\partial x} \\\\\n",
    "&= \\left({-{e^c \\over {2\\sigma^2}} \\cdot 2a}\\right){\\partial a \\over \\partial x} \\\\\n",
    "&= \\frac {-ae^c}{\\sigma^2} \\cdot 1  \\\\\n",
    "&= \\frac {- (x-u)exp(-\\frac{1}{2\\sigma^2}(x-u)^2)}{\\sigma^2} \n",
    "\\end{aligned}\n",
    "$$\n"
   ]
  },
  {
   "cell_type": "markdown",
   "metadata": {},
   "source": [
    "\n",
    "## 5.4\n",
    "$$\n",
    "f'(x) = cos(x) - sin(x) \\\\\n",
    "f''(x) = -sin(x) - cos(x) \\\\\n",
    "f^{'''}(x) = -cos(x) + sin(x) \\\\\n",
    "f^{(4)}(x) = sin(x) + cos(x) \\\\\n",
    "\\vdots\n",
    "$$\n",
    "Thus\n",
    "$$\n",
    "\\begin{aligned}\n",
    "T_n &= f(0) + f'(0) \\cdot x + \\frac{{f''(0)}}{{2!}} \\cdot x^2 + \\frac{{f'''(0)}}{{3!}} \\cdot x^3 + \\frac{{f^{(4)}(0)}}{{4!}} \\cdot x^4 + \\frac{{f^{(5)}(0)}}{{5!}} \\cdot x^5 \\\\\n",
    "&= 1 + x - \\frac{1}{2}x^2 - \\frac{1}{6}x^3 + \\frac{1}{4!}x^4 + \\frac{1}{5!}x^5\n",
    "\\end{aligned}\n",
    "$$"
   ]
  },
  {
   "cell_type": "markdown",
   "metadata": {},
   "source": [
    "## 5.5\n",
    "### a.\n",
    "The dimensions are: \n",
    "\n",
    "${\\partial f_1 \\over \\partial x} = \\begin{bmatrix}\n",
    "{\\partial f_1 \\over \\partial x_1}&{\\partial f_1 \\over \\partial x_2}\n",
    "\\end{bmatrix}$ with dimension $1 \\times 2$\n",
    "\n",
    "${\\partial f_2 \\over \\partial x} = \\begin{bmatrix}\n",
    "{\\partial f_2 \\over \\partial x_1}&{\\partial f_2 \\over \\partial x_2}& \\dots & {\\partial f_2 \\over \\partial x_n}\n",
    "\\end{bmatrix}$ with dimension $1 \\times n$\n",
    "\n",
    "${\\partial f_3 \\over \\partial x} = \\begin{bmatrix}\n",
    "{\\partial f_3 \\over \\partial x_1}&{\\partial f_3 \\over \\partial x_2}& \\dots & {\\partial f_3 \\over \\partial x_n}\n",
    "\\end{bmatrix}$ This is an $(n \\times n) \\times n$ tensor as each ${\\partial f_3 \\over \\partial x_i}$ is $n \\times n$ for $i = 1, 2,...,n$\n",
    "\n",
    "b. \n",
    "$$\n",
    "{\\partial f_1 \\over \\partial x} = \\begin{bmatrix}\n",
    "{cos(x_1)cos(x_2)}&-sin(x_1)sin(x_2)\n",
    "\\end{bmatrix}\n",
    "$$\n",
    "$$\n",
    "{\\partial f_2 \\over \\partial x} = \\begin{bmatrix}\n",
    "{y_1}& y_2 & \\dots & y_n \n",
    "\\end{bmatrix} = y^T\n",
    "$$\n",
    "\n",
    "$f_3$: Let $f_3(x) = K = xx^T =  \\begin{bmatrix} x_1^2 & x_1x_2 & x_1x_3 \\\\\n",
    "    x_2x_1 & x_2^2 & x_2x_3 \\\\\n",
    "    x_3x_1 & x_3x_2 & x_3^2 \\end{bmatrix}\\in \\R ^{n\\times n} $\n",
    "\n",
    "We see that $K_{pq} = x_px_q$, so \n",
    "$\n",
    "{\\partial K_{pq} \\over \\partial x_i} = \\lambda_{pqi}\n",
    "$ where $\\lambda_{pqi} = \\begin{cases}\n",
    "    2x_{i}, & \\text{i=q=p}\\\\\n",
    "    x_p, & p \\neq q, i = q\\\\\n",
    "    x_q, & p \\neq q, i = p\\\\\n",
    "    0,              & \\text{else}\n",
    "\\end{cases}$\n",
    "\n",
    "We see that $\\frac{\\partial K}{\\partial x}$ has dimension $(n \\times n) \\times n$ where each entry is given by $\\lambda_{pqi}$ with $p, q, i = 1, 2, \\dots, n$.\n"
   ]
  },
  {
   "cell_type": "markdown",
   "metadata": {},
   "source": [
    "## 5.6\n",
    "$$\n",
    "\\begin{aligned}\n",
    "\\frac{\\partial f}{\\partial t} &= \\begin{bmatrix}\n",
    "{\\partial f \\over \\partial t_1}&{\\partial f \\over \\partial t_2}& \\dots & {\\partial f \\over \\partial t_n}\n",
    "\\end{bmatrix}_{1 \\times D} \\\\\n",
    "&= cos(log(t^Tt))\\cdot \\frac{1}{t^Tt} \\cdot \\begin{bmatrix} 2t_1 & 2t_2 & \\dots & 2t_n\n",
    "\\end{bmatrix} \\quad \\quad \\text{*using chain rule}\\\\\n",
    "&= 2 cos(log(t^Tt)) \\frac{t^T}{t^Tt}\n",
    "\\end{aligned}\n",
    "$$\n",
    "\n",
    "$\\frac{\\partial g}{\\partial x}$: Let $M = g(X)$\n",
    "\n",
    "$$\n",
    "A = \\begin{bmatrix}\n",
    "    a_{11} & a_{12} & \\cdots & a_{1E} \\\\\n",
    "    a_{21} & a_{22} & \\cdots & a_{2E} \\\\\n",
    "    \\vdots & \\vdots & \\ddots & \\vdots \\\\\n",
    "    a_{D1} & a_{D2} & \\cdots & a_{DE}\n",
    "\\end{bmatrix}, \n",
    "X = \\begin{bmatrix}\n",
    "    x_{11} & x_{12} & \\cdots & x_{1F} \\\\\n",
    "    x_{21} & x_{22} & \\cdots & x_{2F} \\\\\n",
    "    \\vdots & \\vdots & \\ddots & \\vdots \\\\\n",
    "    x_{E1} & x_{E2} & \\cdots & x_{EF}\n",
    "\\end{bmatrix},\n",
    "B = \\begin{bmatrix}\n",
    "    b_{11} & b_{12} & \\cdots & b_{1D} \\\\\n",
    "    b_{21} & b_{22} & \\cdots & b_{2D} \\\\\n",
    "    \\vdots & \\vdots & \\ddots & \\vdots \\\\\n",
    "    b_{F1} & b_{F2} & \\cdots & b_{FD}\n",
    "\\end{bmatrix}\n",
    "$$\n",
    "\n",
    "$$\n",
    "\\begin{aligned}\n",
    "AXB &= \n",
    "\\begin{bmatrix}\n",
    "    \\sum_{k=1}^{E} a_{1k}x_{k1} & \\sum_{k=1}^{E} a_{1k}x_{k2} & \\cdots & \\sum_{k=1}^{E} a_{1k}x_{kF} \\\\\n",
    "    \\sum_{k=1}^{E} a_{2k}x_{k1} & \\sum_{k=1}^{E} a_{2k}x_{k2} & \\cdots & \\sum_{k=1}^{E} a_{2k}x_{kF} \\\\\n",
    "    \\vdots & \\vdots & \\ddots & \\vdots \\\\\n",
    "    \\sum_{k=1}^{E} a_{Dk}x_{k1} & \\sum_{k=1}^{E} a_{Dk}x_{k2} & \\cdots & \\sum_{k=1}^{E} a_{Dk}x_{kF} \n",
    "\\end{bmatrix}\n",
    "\\begin{bmatrix}\n",
    "    b_{11} & b_{12} & \\cdots & b_{1D} \\\\\n",
    "    b_{21} & b_{22} & \\cdots & b_{2D} \\\\\n",
    "    \\vdots & \\vdots & \\ddots & \\vdots \\\\\n",
    "    b_{F1} & b_{F2} & \\cdots & b_{FD}\n",
    "\\end{bmatrix} \\\\\n",
    "&= \\begin{bmatrix}\n",
    "    \\sum_{j=1}^{F}\\sum_{k=1}^{E} a_{1k}x_{kj}b_{j1} &  &  &  \\\\\n",
    "     & \\sum_{j=1}^{F}\\sum_{k=1}^{E} a_{2k}x_{kj}b_{j2} &  &  \\\\\n",
    "     &  & \\ddots &  \\\\\n",
    "     &  &  & \\sum_{j=1}^{F}\\sum_{k=1}^{E} a_{Dk}x_{kj}b_{jd} \n",
    "\\end{bmatrix}\n",
    "\\end{aligned}\n",
    "$$\n",
    "\n",
    "Then \n",
    "$$\n",
    "\\begin{aligned}\n",
    "tr(AXB) &= tr\\left(\\begin{bmatrix}\n",
    "    \\sum_{j=1}^{F}\\sum_{k=1}^{E} a_{1k}x_{kj}b_{j1} &  &  &  \\\\\n",
    "     & \\sum_{j=1}^{F}\\sum_{k=1}^{E} a_{2k}x_{kj}b_{j2} &  &  \\\\\n",
    "     &  & \\ddots &  \\\\\n",
    "     &  &  & \\sum_{j=1}^{F}\\sum_{k=1}^{E} a_{Dk}x_{kj}b_{jd} \n",
    "\\end{bmatrix} \\right) \\\\\n",
    "&= \\sum_{l}^D\\sum_{j}^{F}\\sum_{k}^{E} a_{lk}x_{kj}b_{jl} \\\\\n",
    "&= \\sum_{l}^D\\sum_{j}^{F}(a_{l1}x_{1j}b_{jl}+a_{l2}x_{2j}b_{jl} + \\cdots + a_{le}x_{ej}b_{jl}) \\\\\n",
    "&= \\sum_{l}^D(a_{l1}x_{11}b_{1l}+a_{l2}x_{21}b_{1l} + \\cdots + a_{le}x_{e1}b_{1l}) + (a_{l1}x_{12}b_{2l}+a_{l2}x_{22}b_{2l} + \\cdots + a_{le}x_{e2}b_{2l}) + \\cdots\n",
    "\\end{aligned}\n",
    "$$\n",
    "We see that for each $\\frac{\\partial M}{\\partial x_{ij}}$, only one term in $tr(AXB)$ contains $x_{ij}$: $\\sum_{l}^Da_{li}x_{ij}b_{jl}$. Therefore\n",
    "$$\n",
    "\\frac{\\partial M}{\\partial x_{ij}} = \\sum_{l}^Da_{li}b_{jl} \\quad \\quad \\frac{\\partial M}{\\partial x}= (BA)^T\n",
    "$$"
   ]
  },
  {
   "cell_type": "markdown",
   "metadata": {},
   "source": [
    "\n",
    "## 5.7\n",
    "### a. \n",
    "$$\n",
    "\\begin{aligned}\n",
    "{\\partial f \\over \\partial x} &= {\\partial f \\over \\partial z}{\\partial z \\over \\partial x} \\quad \\quad \\quad \\text{where } {\\partial f \\over \\partial z} \\in \\R \\text{ and }{\\partial z \\over \\partial x} \\text{ has dimension 1xD}\\\\\n",
    "&= {1\\over {1+z}}{\\begin{bmatrix}\n",
    "    2x_1& 2x_2 & \\dots & 2x_D \\\\\n",
    "\\end{bmatrix} }  \\\\\n",
    "&= {{1\\over {1+x^Tx}} \\cdot {2x^T}} \\\\\n",
    "&= \\frac{2x^T}{{1 + x^Tx}}\n",
    "\\end{aligned}\n",
    "$$\n",
    "\n",
    "### b.\n",
    "$$\n",
    "{\\partial f \\over \\partial z} = cos(z) = \n",
    "\\begin{bmatrix}\n",
    "  \\cos(z_1) & 0 & \\cdots & 0 \\\\\n",
    "  0 & \\cos(z_2) & \\cdots & 0 \\\\\n",
    "  \\vdots & \\vdots & \\ddots & \\vdots \\\\\n",
    "  0 & 0 & \\cdots & \\cos(z_e)\n",
    "\\end{bmatrix}_{E \\times E}\n",
    "$$\n",
    "\n",
    "${\\partial z \\over \\partial x}$: We know that $z_i = \\sum_{j=1}^{D} a_{ij} x_j + b_i$, then ${\\partial z_i \\over \\partial x_j} = a_{ij}$. So\n",
    "$$\n",
    "{\\partial z \\over \\partial x} = A \n",
    "$$\n",
    "\n",
    "Finally using chain rule:\n",
    "$$\n",
    "\\begin{aligned} {\\partial f \\over \\partial x} &= {\\partial f \\over \\partial z}{\\partial z \\over \\partial x} \\\\\n",
    "&= cos(Ax + b) \\cdot A \\text{ with dimension }E \\times D\n",
    "\\end {aligned}\n",
    "$$ \n"
   ]
  },
  {
   "cell_type": "markdown",
   "metadata": {},
   "source": [
    "## 5.8 \n",
    "### a.\n",
    "$$\n",
    "\\frac{df}{dz} = -0.5\\exp(-0.5z)\n",
    "$$\n",
    "As $z = y^T S^{-1} y$, we have:\n",
    "\n",
    "$$\n",
    " y^T S^{-1} = \\begin{bmatrix}\n",
    "y_1 & y_2 & \\dots & y_D\n",
    "\\end{bmatrix}\n",
    "\\begin{bmatrix}\n",
    "(S^{-1})_{11} & (S^{-1})_{12} & \\dots & (S^{-1})_{1D} \\\\\n",
    "(S^{-1})_{21} & (S^{-1})_{22} & \\dots & (S^{-1})_{2D} \\\\\n",
    "\\vdots & \\vdots & \\ddots & \\vdots \\\\\n",
    "(S^{-1})_{D1} & (S^{-1})_{D2} & \\dots & (S^{-1})_{DD}\n",
    "\\end{bmatrix}  $$\n",
    "We can find the $i$-th component of $y^T S^{-1}$ is $\\sum_{j=1}^{D} y_j (S^{-1})_{ji} \\quad \\text{for } i = 1, 2, \\ldots, D \\\n",
    "$\n",
    "\n",
    "Then\n",
    "\n",
    "$$ z = \\sum_{i=1}^{D} (y^T S^{-1})_i y_i = \\sum_{i=1}^{D} \\left( \\sum_{j=1}^{D} y_j (S^{-1})_{ji} \\right) y_i \n",
    "$$\n",
    "\n",
    "Then we could find $\\frac{dz}{dy_k}$ for each component $y_k$ of $y$ by evaluating cases where $k = i$ or $k = j$, and putting them together in a vector to get $\\frac{dz}{dy}$. However, it is easier to simply apply formula (5.107) to get \n",
    "\n",
    "$$\n",
    "\\frac{dz}{dy} = y^T(S^{-1} + (S^{-1})^T)\n",
    "$$\n",
    "    \n",
    "**parts of the matrix operations are generated by ChatGPT 3.5*\n",
    "\n",
    "Lastly: \n",
    "$$\n",
    "\\frac{dy}{dx} = \n",
    "\\begin{bmatrix}\n",
    "\\frac{{\\partial y_1}}{{\\partial x_1}} & \\frac{{\\partial y_1}}{{\\partial x_2}} & \\dots & \\frac{{\\partial y_1}}{{\\partial x_D}} \\\\\n",
    "\\frac{{\\partial y_2}}{{\\partial x_1}} & \\frac{{\\partial y_2}}{{\\partial x_2}} & \\dots & \\frac{{\\partial y_2}}{{\\partial x_D}} \\\\\n",
    "\\vdots & \\vdots & \\ddots & \\vdots \\\\\n",
    "\\frac{{\\partial y_D}}{{\\partial x_1}} & \\frac{{\\partial y_D}}{{\\partial x_2}} & \\dots & \\frac{{\\partial y_D}}{{\\partial x_D}}\n",
    "\\end{bmatrix} = I_{D}\n",
    "$$\n",
    "\n",
    "So \n",
    "$$\n",
    "\\frac{df}{dx} = -\\frac{1}{2}exp(-\\frac{1}{2}z)y^T(S^{-1} + (S^{-1})^T)\n",
    "$$\n",
    "\n",
    "### b.\n",
    "\n",
    "$$ \n",
    "XX^T = \\begin{bmatrix}\n",
    "(x_1)^2 & x_1 \\cdot x_2 & \\cdots & x_1 \\cdot x_D \\\\\n",
    "x_2 \\cdot x_1 & (x_2)^2 & \\cdots & x_2 \\cdot x_D \\\\\n",
    "\\vdots & \\vdots & \\ddots & \\vdots \\\\\n",
    "x_D \\cdot x_1 & x_D \\cdot x_2 & \\cdots & (x_D)^2 \\\\\n",
    "\\end{bmatrix}$$\n",
    "\n",
    "$$\n",
    "\\begin{aligned}\n",
    "y &= f(x) \\\\ \n",
    "&= tr\\left( \n",
    "\\begin{bmatrix}\n",
    "(x_1)^2 & x_1 \\cdot x_2 & \\cdots & x_1 \\cdot x_D \\\\\n",
    "x_2 \\cdot x_1 & (x_2)^2 & \\cdots & x_2 \\cdot x_D \\\\\n",
    "\\vdots & \\vdots & \\ddots & \\vdots \\\\\n",
    "x_D \\cdot x_1 & x_D \\cdot x_2 & \\cdots & (x_D)^2 \\\\\n",
    "\\end{bmatrix} + \\begin{bmatrix}\n",
    "\\sigma^2 & 0 & \\cdots & 0 \\\\\n",
    "0 & \\sigma^2 & \\cdots & 0 \\\\\n",
    "\\vdots & \\vdots & \\ddots & \\vdots \\\\\n",
    "0 & 0 & \\cdots & \\sigma^2 \\\\\n",
    "\\end{bmatrix}\n",
    "\\right) \\\\\n",
    "&=  D\\sigma^2 + \\sum_{i=1}^D{x_i}^2\n",
    "\\end{aligned}\n",
    "$$\n",
    "\n",
    "Hence \n",
    "$$\n",
    "\\frac{\\partial y}{\\partial x} = \\begin{bmatrix} 2x_1 & 2x_2 & \\dots & 2x_d \n",
    "\\end{bmatrix}\n",
    " = 2x^T\n",
    "$$\n",
    "\n",
    "### c. \n",
    "$$\n",
    "\\frac{{df}}{{dz}} = \\begin{bmatrix}\n",
    "    \\text{sech}^2(z_1) & 0 & \\cdots & 0 \\\\\n",
    "    0 & \\text{sech}^2(z_2) & \\cdots & 0 \\\\\n",
    "    \\vdots & \\vdots & \\ddots & \\vdots \\\\\n",
    "    0 & 0 & \\cdots & \\text{sech}^2(z_m)\n",
    "\\end{bmatrix}_{M \\times M}\n",
    "$$\n",
    "$$\n",
    "\\frac{{dz}}{{dx}} = A_{M \\times N}\n",
    "$$"
   ]
  },
  {
   "cell_type": "markdown",
   "metadata": {},
   "source": [
    "## 5.9\n",
    "Let $l = log (p(x,z))$, $m = log(q(z, v))$, then $g(x, z, v) = l - m$. \n",
    "\n",
    "Using intermediate variables and flow chart:  \n",
    "$$ l = log(o) \\quad \\quad m = log(k)$$\n",
    "$$ o = p(x, z) \\quad \\quad k = q(z, v)$$\n",
    "$$z = t(e, v)$$\n",
    "![5.9](../Images/Untitled.jpg)\n",
    "\n",
    "By chain rule:\n",
    "$$\n",
    "\\begin{aligned}\n",
    "{\\partial g \\over \\partial v} &= {\\partial g \\over \\partial l}{\\partial l \\over \\partial o}{\\partial o \\over \\partial z}{\\partial z \\over \\partial v} - {\\partial g \\over \\partial m}{\\partial m \\over \\partial k}{\\partial k \\over \\partial v}\\\\\n",
    "&= 1 \\cdot \\frac{1}{o} \\cdot p'(x, z) \\cdot t'(e,v) - 1 \\cdot \\frac{1}{k} \\cdot q'(z, v) \\cdot t'(e, v) \\\\\n",
    "&= \\frac{p'(x,t(e,\\nu))\\cdot t'(e,\\nu) }{p(x,t(e,\\nu))} - \\frac{q'(t(e,\\nu),\\nu)\\cdot t'(e,\\nu)}{q(t(e,\\nu),\\nu)}\n",
    "\\end{aligned}\n",
    "$$\n"
   ]
  },
  {
   "cell_type": "markdown",
   "metadata": {},
   "source": []
  }
 ],
 "metadata": {
  "kernelspec": {
   "display_name": "Python 3.9.12 ('base')",
   "language": "python",
   "name": "python3"
  },
  "language_info": {
   "codemirror_mode": {
    "name": "ipython",
    "version": 3
   },
   "file_extension": ".py",
   "mimetype": "text/x-python",
   "name": "python",
   "nbconvert_exporter": "python",
   "pygments_lexer": "ipython3",
   "version": "3.9.12"
  },
  "orig_nbformat": 4,
  "vscode": {
   "interpreter": {
    "hash": "162b6b064e165ad366d1bd4cdc631c4691b039cb551eb2d47403b16e997dbe09"
   }
  }
 },
 "nbformat": 4,
 "nbformat_minor": 2
}
